examples/steel_wip/Memory.fsti
@@ -5,13 +5,63 @@ let perm =
     FStar.Real.(0.0R <. r && r <=. 1.0R)
   }
 
+/// Abstract type of memories
 val mem  : Type u#1
+
+/// A memory maps a reference to its associated value
 val ref (a:Type u#0) : Type u#0
 
+/// A predicate describing non-overlapping memories
 val disjoint (m0 m1:mem) : prop
+
+/// disjointness is symmetric
+val disjoint_sym (m0 m1:mem)
+  : Lemma (disjoint m0 m1 <==> disjoint m1 m0)
+
+/// disjoint memories can be combined
 val join (m0:mem) (m1:mem{disjoint m0 m1}) : mem
 
+/// disjointness distributes over join
+val disjoint_join (m0 m1 m2:mem)
+  : Lemma (disjoint m1 m2 /\
+           disjoint m0 (join m1 m2) ==>
+           disjoint m0 m1 /\
+           disjoint m0 m2 /\
+           disjoint (join m0 m1) m2 /\
+           disjoint (join m0 m2) m1)
+
+val join_commutative (m0 m1:mem)
+  : Lemma
+    (requires
+      disjoint m0 m1)
+    (ensures
+      (disjoint_sym m0 m1;
+       join m0 m1 == join m1 m0))
+
+val join_associative (m0 m1 m2:mem)
+  : Lemma
+    (requires
+      disjoint m1 m2 /\
+      disjoint m0 (join m1 m2))
+    (ensures
+      (disjoint_join m0 m1 m2;
+       join m0 (join m1 m2) == join (join m0 m1) m2))
+
+/// The type of heap assertions
 val hprop : Type u#1
+/// interpreting heap assertions as memory predicates
+val interp (p:hprop) (m:mem) : prop
+
+/// A common abbreviation: memories validating p
+let hmem (p:hprop) = m:mem{interp p m}
+
+/// Equivalence relation on hprops is just
+/// equivalence of their interpretations
+let equiv (p1 p2:hprop) =
+  forall m. interp p1 m <==> interp p2 m
+
+/// All the standard connectives of separation logic
+val emp : hprop
 val pts_to (#a:_) (r:ref a) (p:perm) (v:a) : hprop
 val h_and (p1 p2:hprop) : hprop
 val h_or  (p1 p2:hprop) : hprop
@@ -20,17 +70,18 @@ val wand  (p1 p2:hprop) : hprop
 val h_exists (#a:Type0) (f: (a -> hprop)) : hprop
 val h_forall (#a:Type0) (f: (a -> hprop)) : hprop
 
+////////////////////////////////////////////////////////////////////////////////
+// pts_to and abbreviations
+//////////////////////////////////////////////////////////////////////////////////////////
 let ptr_perm #a (r:ref a) (p:perm) =
     h_exists (fun v -> pts_to r p v)
 
 let ptr #a (r:ref a) =
     h_exists (fun p -> ptr_perm r p)
 
-val interp (p:hprop) (m:mem) : prop
-let hmem (p:hprop) = m:mem{interp p m}
-let equiv (p1 p2:hprop) =
-  forall m. interp p1 m <==> interp p2 m
-
+////////////////////////////////////////////////////////////////////////////////
+// star
+////////////////////////////////////////////////////////////////////////////////
 val star_commutative (p1 p2:hprop)
   : Lemma ((p1 `star` p2) `equiv` (p2 `star` p1))
 val star_associative (p1 p2 p3:hprop)
@@ -38,36 +89,119 @@ val star_associative (p1 p2 p3:hprop)
            `equiv`
            ((p1 `star` p2) `star` p3))
 
+////////////////////////////////////////////////////////////////////////////////
+// Actions:
+// sel, split, update
+////////////////////////////////////////////////////////////////////////////////
 val sel (#a:_) (r:ref a) (m:hmem (ptr r))
   : a
 
+/// sel respect pts_to
 val sel_lemma (#a:_) (r:ref a) (p:perm) (m:hmem (ptr_perm r p))
   : Lemma (interp (ptr r) m /\
            interp (pts_to r p (sel r m)) m)
 
+/// memories satisfying [p1 `star` p2] can be split
+/// into disjoint fragments satisfying each of them
 val split_mem (p1 p2:hprop) (m:hmem (p1 `star` p2))
   : Tot (ms:(hmem p1 & hmem p2){
             let m1, m2 = ms in
             disjoint m1 m2 /\
             m == join m1 m2})
 
+/// upd requires a full permission
+/// it respects frames
 val upd (#a:_) (r:ref a) (v:a)
         (frame:hprop)
         (m:hmem (ptr_perm r 1.0R  `star` frame))
   : Tot (m:hmem (pts_to r 1.0R v `star` frame))
 
-val intro_wand (p1 p2:hprop) (m:mem)
+////////////////////////////////////////////////////////////////////////////////
+// wand
+////////////////////////////////////////////////////////////////////////////////
+
+/// A low-level introduction form for wand in terms of disjoint
+val intro_wand_alt (p1 p2:hprop) (m:mem)
   : Lemma
     (requires
       (forall (m0:hmem p1).
-         disjoint m0 m /\
+         disjoint m0 m ==>
          interp p2 (join m0 m)))
     (ensures
       interp (wand p1 p2) m)
 
+/// A higher-level introduction for wand as a cut
+val intro_wand (p q r:hprop) (m:hmem q)
+  : Lemma
+    (requires
+      (forall (m:hmem (p `star` q)). interp r m))
+    (ensures
+      interp (p `wand` r) m)
+
+/// Standard wand elimination
 val elim_wand (p1 p2:hprop) (m:mem)
   : Lemma
     (requires
       (interp ((p1 `wand` p2) `star` p1) m))
     (ensures
       interp p2 m)
+
+////////////////////////////////////////////////////////////////////////////////
+// or
+////////////////////////////////////////////////////////////////////////////////
+val intro_or_l (p1 p2:hprop) (m:hmem p1)
+  : Lemma (interp (h_or p1 p2) m)
+
+val intro_or_r (p1 p2:hprop) (m:hmem p2)
+  : Lemma (interp (h_or p1 p2) m)
+
+/// star can be factored out of or
+val or_star (p1 p2 p:hprop) (m:hmem ((p1 `star` p) `h_or` (p2 `star` p)))
+  : Lemma (interp ((p1 `h_or` p2) `star` p) m)
+
+/// A standard or eliminator
+val elim_or (p1 p2 q:hprop) (m:hmem (p1 `h_or` p2))
+  : Lemma (((forall (m:hmem p1). interp q m) /\
+            (forall (m:hmem p2). interp q m)) ==> interp q m)
+
+
+////////////////////////////////////////////////////////////////////////////////
+// and
+////////////////////////////////////////////////////////////////////////////////
+val intro_and (p1 p2:hprop) (m:mem)
+  : Lemma (interp p1 m /\
+           interp p2 m ==>
+           interp (p1 `h_and` p2) m)
+
+val elim_and (p1 p2:hprop) (m:hmem (p1 `h_and` p2))
+  : Lemma (interp p1 m /\
+           interp p2 m)
+
+////////////////////////////////////////////////////////////////////////////////
+// h_exists
+////////////////////////////////////////////////////////////////////////////////
+
+val intro_exists (#a:_) (x:a) (p : a -> hprop) (m:hmem (p x))
+  : Lemma (interp (h_exists p) m)
+
+val elim_exists (#a:_) (p:a -> hprop) (q:hprop) (m:hmem (h_exists p))
+  : Lemma
+    ((forall (x:a). interp (p x) m ==> interp q m) ==>
+     interp q m)
+
+
+////////////////////////////////////////////////////////////////////////////////
+// h_forall
+////////////////////////////////////////////////////////////////////////////////
+
+val intro_forall (#a:_) (p : a -> hprop) (m:mem)
+  : Lemma ((forall x. interp (p x) m) ==> interp (h_forall p) m)
+
+val elim_forall (#a:_) (p : a -> hprop) (m:hmem (h_forall p))
+  : Lemma ((forall x. interp (p x) m) ==> interp (h_forall p) m)
+
+////////////////////////////////////////////////////////////////////////////////
+// emp
+////////////////////////////////////////////////////////////////////////////////
+val intro_emp (m:mem)
+  : Lemma (interp emp m)
